array get(arr, key) is proven

coq/assoc.c
@@ -5,7 +5,8 @@
 
 int get(int* arr, int key)
 {
-    return arr[key];
+    int rez = arr[key]; //using memory access (arr[key]) in an expression
+    return rez; // (return ...) is forbidden by VST.
 }
 
 void set(int* arr, int key, int val)
